Weidenbach_Book/IsaSAT/IsaSAT_Setup3_LLVM.thy
@@ -1,0 +1,138 @@
+theory IsaSAT_Setup3_LLVM
+  imports IsaSAT_Setup IsaSAT_Watch_List_LLVM IsaSAT_Lookup_Conflict_LLVM
+    More_Sepref.WB_More_Refinement IsaSAT_Clauses_LLVM LBD_LLVM
+    IsaSAT_Options_LLVM IsaSAT_VMTF_Setup_LLVM
+    IsaSAT_Arena_Sorting_LLVM
+    IsaSAT_Rephase_LLVM
+    IsaSAT_EMA_LLVM
+    IsaSAT_Stats_LLVM
+    IsaSAT_Setup0_LLVM
+begin
+
+sepref_def wasted_bytes_st_impl
+  is \<open>RETURN o wasted_bytes_st\<close>
+  :: \<open>isasat_bounded_assn\<^sup>k \<rightarrow>\<^sub>a word64_assn\<close>
+  supply [[goals_limit=1]]
+  unfolding isasat_bounded_assn_def
+    heuristic_assn_def wasted_bytes_st_def
+  by sepref
+
+
+lemma id_unat[sepref_fr_rules]:
+   \<open>(return o id, RETURN o unat) \<in> word32_assn\<^sup>k \<rightarrow>\<^sub>a uint32_nat_assn\<close>
+  apply sepref_to_hoare
+  apply vcg
+  by (auto simp: ENTAILS_def unat_rel_def unat.rel_def br_def pred_lift_merge_simps
+     pred_lift_def pure_true_conv)
+
+sepref_register set_zero_wasted mop_save_phase_heur add_lbd
+
+
+sepref_def add_lbd_impl
+  is \<open>uncurry (RETURN oo add_lbd)\<close>
+  :: \<open>word32_assn\<^sup>k *\<^sub>a stats_assn\<^sup>d \<rightarrow>\<^sub>a stats_assn\<close>
+  supply [[goals_limit=1]]
+  unfolding add_lbd_def
+  by sepref
+
+
+sepref_register isa_trail_nth isasat_trail_nth_st
+
+sepref_def isasat_trail_nth_st_code
+  is \<open>uncurry isasat_trail_nth_st\<close>
+  :: \<open>isasat_bounded_assn\<^sup>k *\<^sub>a sint64_nat_assn\<^sup>k \<rightarrow>\<^sub>a unat_lit_assn\<close>
+  supply [[goals_limit=1]]
+  unfolding isasat_trail_nth_st_alt_def isasat_bounded_assn_def
+  by sepref
+
+sepref_def heuristic_reluctant_triggered2_st_impl
+  is \<open>RETURN o heuristic_reluctant_triggered2_st\<close>
+  :: \<open>isasat_bounded_assn\<^sup>k \<rightarrow>\<^sub>a bool1_assn\<close>
+  unfolding heuristic_reluctant_triggered2_st_def isasat_bounded_assn_def
+  by sepref
+
+sepref_def heuristic_reluctant_untrigger_st_impl
+  is \<open>RETURN o heuristic_reluctant_untrigger_st\<close>
+  :: \<open>isasat_bounded_assn\<^sup>d \<rightarrow>\<^sub>a isasat_bounded_assn\<close>
+  unfolding heuristic_reluctant_untrigger_st_def isasat_bounded_assn_def
+    fold_tuple_optimizations
+  by sepref
+
+
+sepref_register incr_restart_stat
+
+
+sepref_register clss_size_lcountUE clss_size_lcountUS learned_clss_count clss_size_allcount
+
+sepref_def incr_restart_stat_fast_code
+  is \<open>incr_restart_stat\<close>
+  :: \<open>isasat_bounded_assn\<^sup>d \<rightarrow>\<^sub>a isasat_bounded_assn\<close>
+  supply [[goals_limit=1]]
+  unfolding incr_restart_stat_def isasat_bounded_assn_def PR_CONST_def
+    heuristic_assn_def fold_tuple_optimizations
+  by sepref
+
+sepref_register incr_lrestart_stat clss_size_decr_lcount
+    clss_size_incr_lcountUE clss_size_incr_lcountUS
+
+sepref_def incr_lrestart_stat_fast_code
+  is \<open>incr_lrestart_stat\<close>
+  :: \<open>isasat_bounded_assn\<^sup>d \<rightarrow>\<^sub>a isasat_bounded_assn\<close>
+  supply [[goals_limit=1]]
+  unfolding incr_lrestart_stat_def isasat_bounded_assn_def PR_CONST_def
+    heuristic_assn_def fold_tuple_optimizations
+  by sepref
+
+sepref_register mark_unused_st_heur
+sepref_def mark_unused_st_fast_code
+  is \<open>uncurry (RETURN oo mark_unused_st_heur)\<close>
+  :: \<open>[\<lambda>(C, S). arena_act_pre (get_clauses_wl_heur S) C]\<^sub>a
+        sint64_nat_assn\<^sup>k *\<^sub>a isasat_bounded_assn\<^sup>d \<rightarrow> isasat_bounded_assn\<close>
+  unfolding mark_unused_st_heur_def isasat_bounded_assn_def
+    arena_act_pre_mark_used[intro!] fold_tuple_optimizations
+  supply [[goals_limit = 1]]
+  by sepref
+
+sepref_def mop_mark_unused_st_heur_impl
+  is \<open>uncurry mop_mark_unused_st_heur\<close>
+  :: \<open> sint64_nat_assn\<^sup>k *\<^sub>a isasat_bounded_assn\<^sup>d \<rightarrow>\<^sub>a isasat_bounded_assn\<close>
+  unfolding mop_mark_unused_st_heur_def fold_tuple_optimizations
+  by sepref
+
+
+sepref_register get_the_propagation_reason_pol_st
+
+sepref_def get_the_propagation_reason_pol_st_code
+  is \<open>uncurry get_the_propagation_reason_pol_st\<close>
+  :: \<open>isasat_bounded_assn\<^sup>k *\<^sub>a unat_lit_assn\<^sup>k \<rightarrow>\<^sub>a snat_option_assn' TYPE(64)\<close>
+  supply [[goals_limit=1]]
+  unfolding get_the_propagation_reason_pol_st_alt_def isasat_bounded_assn_def
+  by sepref
+
+sepref_def empty_US_heur_code
+  is \<open>RETURN o empty_US_heur\<close>
+  :: \<open>isasat_bounded_assn\<^sup>d \<rightarrow>\<^sub>a isasat_bounded_assn\<close>
+  unfolding empty_US_heur_def isasat_bounded_assn_def
+  by sepref
+
+lemma current_restart_phase_alt_def:
+  \<open>current_restart_phase = (\<lambda>(fast_ema, slow_ema,
+    (ccount, ema_lvl, restart_phase, end_of_phase), _).
+    restart_phase)\<close>
+  by auto
+
+sepref_def current_restart_phase_impl
+  is \<open>RETURN o current_restart_phase\<close>
+  :: \<open>heuristic_assn\<^sup>k \<rightarrow>\<^sub>a word_assn\<close>
+  unfolding current_restart_phase_alt_def heuristic_assn_def
+  by sepref
+
+
+
+sepref_def get_restart_phase_imp
+  is \<open>(RETURN o get_restart_phase)\<close>
+  :: \<open>isasat_bounded_assn\<^sup>k \<rightarrow>\<^sub>a word_assn\<close>
+  unfolding get_restart_phase_def isasat_bounded_assn_def
+  by sepref
+
+end
